<?xml version="1.0" encoding="UTF-8"?>
<rdf:RDF
   xmlns:owl="http://www.w3.org/2002/07/owl#"
   xmlns:rdf="http://www.w3.org/1999/02/22-rdf-syntax-ns#"
   xmlns:rdfs="http://www.w3.org/2000/01/rdf-schema#"
>
  <rdf:Description rdf:about="http://purl.org/socialparticipation/ot/BigData">
    <rdfs:comment xml:lang="en">Big data is a broad term for data sets so large or complex that traditional data processing applications are inadequate. Challenges include analysis, capture, data curation, search, sharing, storage, transfer, visualization, and information privacy. The term often refers simply to the use of predictive analytics or other certain advanced methods to extract value from data, and seldom to a particular size of data set. Accuracy in big data may lead to more confident decision making. And better decisions can mean greater operational efficiency, cost reductions and reduced risk.</rdfs:comment>
    <rdfs:subClassOf rdf:resource="http://purl.org/socialparticipation/ot/ComputerScience"/>
    <rdf:type rdf:resource="http://www.w3.org/2002/07/owl#Class"/>
    <rdfs:label xml:lang="pt">Megadados</rdfs:label>
    <rdfs:label xml:lang="en">Big Data</rdfs:label>
  </rdf:Description>
  <rdf:Description rdf:about="http://purl.org/socialparticipation/ot/AnthropologicalPhysics">
    <rdfs:subClassOf rdf:resource="http://purl.org/socialparticipation/ot/ComplexNetworksTheory"/>
    <rdfs:label xml:lang="pt">Física Antropológica</rdfs:label>
    <rdf:type rdf:resource="http://www.w3.org/2002/07/owl#Class"/>
    <rdfs:label xml:lang="en">Anthropological Physics</rdfs:label>
    <rdfs:comment xml:lang="en">the complex networks study to benefit the participant.</rdfs:comment>
  </rdf:Description>
  <rdf:Description rdf:about="http://purl.org/socialparticipation/ot/ProbabilityTheory">
    <rdf:type rdf:resource="http://www.w3.org/2002/07/owl#Class"/>
    <rdfs:label xml:lang="pt">Teoria das Probabilidades</rdfs:label>
    <rdfs:comment xml:lang="en">Probability theory is the branch of mathematics concerned with probability, the analysis of random phenomena.[1] The central objects of probability theory are random variables, stochastic processes, and events: mathematical abstractions of non-deterministic events or measured quantities that may either be single occurrences or evolve over time in an apparently random fashion. (wikipedia, Jun/2015)</rdfs:comment>
    <rdfs:label xml:lang="en">Probability Theory</rdfs:label>
  </rdf:Description>
  <rdf:Description rdf:about="http://purl.org/socialparticipation/ot/ComplexNetwork">
    <rdf:type rdf:resource="http://www.w3.org/2002/07/owl#Class"/>
    <rdfs:label xml:lang="pt">Rede Complexa</rdfs:label>
    <rdfs:comment xml:lang="en">The study of complex networks is a young and active area of scientific research inspired largely by the empirical study of real-world networks such as computer networks and social networks. (Wikipedia) 
a frequently big network in the environment or for the consideration of the environment that they reside. (R. Fabbri)</rdfs:comment>
    <rdfs:label xml:lang="en">Complex Network</rdfs:label>
  </rdf:Description>
  <rdf:Description rdf:about="http://purl.org/socialparticipation/ot/ComplexNetworksTheory">
    <rdfs:label xml:lang="en">Complex Networks Theory</rdfs:label>
    <rdfs:label xml:lang="pt">Teoria das Redes Complexas</rdfs:label>
    <rdfs:subClassOf rdf:resource="http://purl.org/socialparticipation/ot/StatisticalPhysics"/>
    <rdf:type rdf:resource="http://www.w3.org/2002/07/owl#Class"/>
    <rdfs:comment xml:lang="en">Complex networks area of scientific research</rdfs:comment>
  </rdf:Description>
  <rdf:Description rdf:about="http://purl.org/socialparticipation/ot/SocialParticipation">
    <rdf:type rdf:resource="http://www.w3.org/2002/07/owl#Class"/>
    <rdfs:comment xml:lang="en">also social engagement or social involvement, social participation refers to one's degree of participation in a community or society.</rdfs:comment>
    <rdfs:label xml:lang="pt">Participação Social</rdfs:label>
    <rdfs:label xml:lang="en">Social Participation</rdfs:label>
  </rdf:Description>
  <rdf:Description rdf:about="http://purl.org/socialparticipation/ot/DataMining">
    <rdf:type rdf:resource="http://www.w3.org/2002/07/owl#Class"/>
    <rdfs:comment xml:lang="en">the computational process of discovering patterns in large data sets involving methods at the intersection of artificial intelligence, machine learning, statistics, and database systems</rdfs:comment>
    <rdfs:label xml:lang="en">Data Mining</rdfs:label>
    <rdfs:label xml:lang="pt">Mineração de Dados</rdfs:label>
  </rdf:Description>
  <rdf:Description rdf:about="http://purl.org/socialparticipation/ot/InteractionNetwork">
    <rdf:type rdf:resource="http://www.w3.org/2002/07/owl#Class"/>
    <rdfs:label xml:lang="en">Interaction Network</rdfs:label>
    <rdfs:comment xml:lang="en">Rede com grafo proveniente de vértices e interações entre pares deles. (R. Fabbri)</rdfs:comment>
    <rdfs:label xml:lang="pt">Rede de Interação</rdfs:label>
    <rdfs:subClassOf rdf:resource="http://purl.org/socialparticipation/ot/RelationshipNetwork"/>
  </rdf:Description>
  <rdf:Description rdf:about="http://purl.org/socialparticipation/ot/LinkedData">
    <rdfs:label xml:lang="pt">Dados Ligados</rdfs:label>
    <rdfs:subClassOf rdf:resource="http://purl.org/socialparticipation/ot/ComputerScience"/>
    <rdf:type rdf:resource="http://www.w3.org/2002/07/owl#Class"/>
    <rdfs:comment xml:lang="en">also known as semantic web, studies methods for publishing structured data so that it can be interlinked and become more useful through semantic queries.</rdfs:comment>
    <rdfs:label xml:lang="en">Linked Data</rdfs:label>
  </rdf:Description>
  <rdf:Description rdf:about="http://purl.org/socialparticipation/ot/Statistics">
    <rdf:type rdf:resource="http://www.w3.org/2002/07/owl#Class"/>
    <rdfs:comment xml:lang="en">The mathematical study of the likelihood and probability of events occurring based on known information and inferred by taking a limited number of samples. (Wolfram)
        Statistics is the science of learning from data, and of measuring, controlling, and communicating uncertainty; and it thereby provides the navigation essential for controlling the course of scientific and societal advances (Davidian, M. and Louis, T. A., 10.1126/science.1218685, adopted by ASA - American Statistical Association.</rdfs:comment>
    <rdfs:label xml:lang="pt">Estatística</rdfs:label>
    <rdfs:label xml:lang="en">Estatistics</rdfs:label>
  </rdf:Description>
  <rdf:Description rdf:about="http://purl.org/socialparticipation/ot/HumanBehavioralEcology">
    <rdf:type rdf:resource="http://www.w3.org/2002/07/owl#Class"/>
    <rdfs:comment xml:lang="en">also known as human evolutionary ecology, HBE applies the principles of evolutionary theory and optimization to the study of human behavioral and cultural diversity.</rdfs:comment>
    <rdfs:subClassOf rdf:resource="http://purl.org/socialparticipation/ot/BiologicalAnthropology"/>
    <rdfs:label xml:lang="pt">Ecologia Behaviorista Humana</rdfs:label>
    <rdfs:label xml:lang="en">Human Behavioral Ecology</rdfs:label>
  </rdf:Description>
  <rdf:Description rdf:about="http://purl.org/socialparticipation/ot/HumanSocialNetwork">
    <rdfs:subClassOf rdf:resource="http://purl.org/socialparticipation/ot/SocialNetwork"/>
    <rdf:type rdf:resource="http://www.w3.org/2002/07/owl#Class"/>
    <rdfs:label xml:lang="pt">Rede Social Humana</rdfs:label>
    <rdfs:label xml:lang="en">Human Social Network</rdfs:label>
    <rdfs:comment xml:lang="en">a social network whoose social actors are human beings.</rdfs:comment>
  </rdf:Description>
  <rdf:Description rdf:about="http://purl.org/socialparticipation/ot/grounds">
    <owl:subPropertyOf rdf:resource="http://purl.org/socialparticipation/ot/enables"/>
    <rdf:type rdf:resource="http://www.w3.org/2002/07/owl#ObjectProperty"/>
    <rdfs:label xml:lang="pt">fundamenta</rdfs:label>
    <rdfs:label xml:lang="en">grounds</rdfs:label>
  </rdf:Description>
  <rdf:Description rdf:about="http://purl.org/socialparticipation/ot/Transdisciplinarity">
    <rdf:type rdf:resource="http://www.w3.org/2002/07/owl#Class"/>
    <rdfs:label xml:lang="en">Transdisciplinarity</rdfs:label>
    <rdfs:comment xml:lang="en">Transdisciplinarity connotes a research strategy that crosses many disciplinary boundaries to create a holistic approach.</rdfs:comment>
    <rdfs:label xml:lang="pt">Transdisciplinaridade</rdfs:label>
  </rdf:Description>
  <rdf:Description rdf:about="http://purl.org/socialparticipation/ot/Human">
    <rdf:type rdf:resource="http://www.w3.org/2002/07/owl#Class"/>
    <rdfs:comment xml:lang="en">the only extant members of the hominini clade of the great apes (the human clade, Homo genus); characterized by erect posture and bipedal locomotion, manual dexterity and increased tool use, and a general trend toward larger, more complex brains and societies.</rdfs:comment>
    <rdfs:label xml:lang="en">Human</rdfs:label>
    <rdfs:label xml:lang="pt">Humano</rdfs:label>
  </rdf:Description>
  <rdf:Description rdf:about="http://purl.org/socialparticipation/ot/RelationshipNetwork">
    <rdf:type rdf:resource="http://www.w3.org/2002/07/owl#Class"/>
    <rdfs:label xml:lang="en">Relationship Network</rdfs:label>
    <rdfs:subClassOf rdf:resource="http://purl.org/socialparticipation/ot/ComplexNetwork"/>
    <rdfs:comment xml:lang="en">Rede com grafo proveniente de vértices e relacionamentos entre pares deles. (R. Fabbri)</rdfs:comment>
    <rdfs:label xml:lang="pt">Rede de Relacionamento</rdfs:label>
  </rdf:Description>
  <rdf:Description rdf:about="http://purl.org/socialparticipation/ot/SocialNetwork">
    <rdf:type rdf:resource="http://www.w3.org/2002/07/owl#Class"/>
    <rdfs:subClassOf rdf:resource="http://purl.org/socialparticipation/ot/RelationshipNetwork"/>
    <rdfs:label xml:lang="pt">Rede Social</rdfs:label>
    <rdfs:label xml:lang="en">Social Network</rdfs:label>
    <rdfs:comment xml:lang="en">a social structure made up of a set of social actors (such as individuals or organizations) and a set of the dyadic ties between these actors.</rdfs:comment>
  </rdf:Description>
  <rdf:Description rdf:about="http://purl.org/socialparticipation/ot/SocioculturalAnthropology">
    <rdf:type rdf:resource="http://www.w3.org/2002/07/owl#Class"/>
    <rdfs:label xml:lang="pt">Antropologia Sociocultural</rdfs:label>
    <rdfs:subClassOf rdf:resource="http://purl.org/socialparticipation/ot/Anthropology"/>
    <rdfs:comment xml:lang="en">used to refer to social anthropology and cultural anthropology together. Cultural anthropology has greater prominance in the USA, and  are holistic, oriented to the ways in which culture affects individual experience and provides a rounded view of the knowledge, customs, and institutions of a people. Social anthropology attempts to isolate a particular system of social relations and provide analytical bases to social life.</rdfs:comment>
    <rdfs:label xml:lang="en">Sociocultural Anthropology</rdfs:label>
  </rdf:Description>
  <rdf:Description rdf:about="http://purl.org/socialparticipation/ot/BiologicalAnthropology">
    <rdfs:label xml:lang="pt">Antropologia Biológica</rdfs:label>
    <rdf:type rdf:resource="http://www.w3.org/2002/07/owl#Class"/>
    <rdfs:label xml:lang="en">Biological Anthropology</rdfs:label>
    <rdfs:comment xml:lang="en">also known as physical anthropology, is a scientific discipline concerned with the biological and behavioral aspects of human beings, their related non-human primates and their extinct hominin ancestors. It is a subfield of anthropology that provides a biological perspective to the systematic study of human beings.</rdfs:comment>
    <rdfs:subClassOf rdf:resource="http://purl.org/socialparticipation/ot/Anthropology"/>
  </rdf:Description>
  <rdf:Description rdf:about="http://purl.org/socialparticipation/ot/ComputationalLinguistics">
    <rdfs:label xml:lang="en">Computational Linguistics</rdfs:label>
    <rdfs:label xml:lang="pt">Linguística Computacional</rdfs:label>
    <rdfs:comment xml:lang="en">an interdisciplinary field concerned with the statistical or rule-based modeling of natural language from a computational perspective.</rdfs:comment>
    <rdf:type rdf:resource="http://www.w3.org/2002/07/owl#Class"/>
    <rdfs:subClassOf rdf:resource="http://purl.org/socialparticipation/ot/ComputerScience"/>
  </rdf:Description>
  <rdf:Description rdf:about="http://purl.org/socialparticipation/ot/SocialPsychology">
    <rdfs:label xml:lang="en">Social Psychology</rdfs:label>
    <rdf:type rdf:resource="http://www.w3.org/2002/07/owl#Class"/>
    <rdfs:comment xml:lang="en">the scientific study of how people's thoughts, feelings, and behaviors are influenced by the actual, imagined, or implied presence of others.</rdfs:comment>
    <rdfs:label xml:lang="pt">Psicologia Social</rdfs:label>
  </rdf:Description>
  <rdf:Description rdf:about="http://purl.org/socialparticipation/ot/GraphTheory">
    <rdf:type rdf:resource="http://www.w3.org/2002/07/owl#Class"/>
    <rdfs:comment xml:lang="en">the study of graphs, which are mathematical structures used to model pairwise relations between objects. (wikipedia, Jun/2015)</rdfs:comment>
    <rdfs:label xml:lang="pt">Teoria dos Grafos</rdfs:label>
    <rdfs:label xml:lang="en">Graph Theory</rdfs:label>
  </rdf:Description>
  <rdf:Description rdf:about="http://purl.org/socialparticipation/ot/related">
    <rdfs:label xml:lang="pt">relacionado</rdfs:label>
    <rdf:type rdf:resource="http://www.w3.org/2002/07/owl#ObjectProperty"/>
    <rdf:type rdf:resource="http://www.w3.org/2002/07/owl#SymmetricProperty"/>
    <rdfs:label xml:lang="en">related</rdfs:label>
  </rdf:Description>
  <rdf:Description rdf:about="http://purl.org/socialparticipation/ot/Sociology">
    <rdf:type rdf:resource="http://www.w3.org/2002/07/owl#Class"/>
    <rdfs:label xml:lang="en">Anthropological Physics</rdfs:label>
    <rdfs:comment xml:lang="en">the study of human social relationships and institutions. (UNC)</rdfs:comment>
    <rdfs:label xml:lang="pt">Sociologia</rdfs:label>
  </rdf:Description>
  <rdf:Description rdf:about="http://purl.org/socialparticipation/ot/StatisticalPhysics">
    <rdf:type rdf:resource="http://www.w3.org/2002/07/owl#Class"/>
    <rdfs:subClassOf rdf:resource="http://purl.org/socialparticipation/ot/Physics"/>
    <rdfs:label xml:lang="pt">Física Estatística</rdfs:label>
    <rdfs:comment xml:lang="en">Branch of physics that uses methods of probability theory and statistics</rdfs:comment>
    <rdfs:label xml:lang="en">Statistical Physics</rdfs:label>
  </rdf:Description>
  <rdf:Description rdf:about="http://purl.org/socialparticipation/ot/Anthropology">
    <rdfs:comment xml:lang="en">the study of humans. Its main subdivisions are cultural anthropology, which describes the workings of societies around the world, and biological anthropology, which concerns long-term development of the human organism.</rdfs:comment>
    <rdf:type rdf:resource="http://www.w3.org/2002/07/owl#Class"/>
    <rdfs:label xml:lang="pt">Antropologia</rdfs:label>
    <rdfs:label xml:lang="en">Anthropology</rdfs:label>
  </rdf:Description>
  <rdf:Description rdf:about="http://purl.org/socialparticipation/ot/enables">
    <rdf:type rdf:resource="http://www.w3.org/2002/07/owl#ObjectProperty"/>
    <rdfs:label xml:lang="pt">possibilita</rdfs:label>
    <rdfs:label xml:lang="en">enables</rdfs:label>
  </rdf:Description>
  <rdf:Description rdf:about="http://purl.org/socialparticipation/ot/composes">
    <rdf:type rdf:resource="http://www.w3.org/2002/07/owl#ObjectProperty"/>
    <rdfs:label xml:lang="pt">compõe</rdfs:label>
    <rdfs:label xml:lang="en">composes</rdfs:label>
  </rdf:Description>
  <rdf:Description rdf:about="http://purl.org/socialparticipation/ot/Physics">
    <rdfs:label xml:lang="pt">Física</rdfs:label>
    <rdf:type rdf:resource="http://www.w3.org/2002/07/owl#Class"/>
    <rdfs:comment xml:lang="en">the natural science that involves the study of matter, its motion through space and time, and related concepts such as energy and force. More broadly, it is the general analysis of nature, conducted in order to understand how the universe behaves.</rdfs:comment>
    <rdfs:comment xml:lang="en">Mathematics is the language used for compact description of the order in nature, especially the laws of physics. This was noted and advocated by Pythagoras, Plato, Galileo, and Newton.
     Physics theories use mathematics to obtain order and provide precise formulas, precise or estimated solutions, quantitative results and predictions. Experiment results in physics are numerical measurements. Technologies based on mathematics, like computation have made computational physics an active area of research.
     Ontology is a prerequisite for physics, but not for mathematics. It means physics is ultimately concerned with descriptions of the real world, while mathematics is concerned with abstract patterns, even beyond the real world. Thus physics statements are synthetic, while mathematical statements are analytic. Mathematics contains hypotheses, while physics contains theories. Mathematics statements have to be only logically true, while predictions of physics statements must match observed and experimental data.</rdfs:comment>
    <rdfs:label xml:lang="en">Physics</rdfs:label>
  </rdf:Description>
  <rdf:Description rdf:about="http://purl.org/socialparticipation/ot/Topology">
    <rdfs:label xml:lang="pt">Topologia</rdfs:label>
    <rdf:type rdf:resource="http://www.w3.org/2002/07/owl#Class"/>
    <rdfs:label xml:lang="en">Topology</rdfs:label>
    <rdfs:comment xml:lang="en">The study of topological spaces. It is an area of mathematics concerned with the properties of space that are preserved under continuous deformations, such as stretching and bending, but not tearing or gluing. Important topological properties include connectedness and compactness. A topological space may be defined as a set of points, along with a set of neighbourhoods for each point, that satisfy a set of axioms relating points and neighbourhoods. The definition of a topological space relies only upon set theory and is the most general notion of a mathematical space that allows for the definition of concepts such as continuity, connectedness, and convergence.[1] Other spaces, such as manifolds and metric spaces, are specializations of topological spaces with extra structures or constraints. Being so general, topological spaces are a central unifying notion and appear in virtually every branch of modern mathematics.</rdfs:comment>
  </rdf:Description>
  <rdf:Description rdf:about="http://purl.org/socialparticipation/ot/dealsWith">
    <rdf:type rdf:resource="http://www.w3.org/2002/07/owl#ObjectProperty"/>
    <rdfs:label xml:lang="pt">trata de</rdfs:label>
    <rdfs:label xml:lang="en">deals with</rdfs:label>
  </rdf:Description>
  <rdf:Description rdf:about="http://purl.org/socialparticipation/ot/ComputerScience">
    <rdfs:comment xml:lang="en">the scientific and practical approach to computation and its applications.</rdfs:comment>
    <rdf:type rdf:resource="http://www.w3.org/2002/07/owl#Class"/>
    <rdfs:label xml:lang="pt">Ciência da Computação</rdfs:label>
    <rdfs:label xml:lang="en">Computer Science</rdfs:label>
  </rdf:Description>
  <rdf:Description rdf:about="http://purl.org/socialparticipation/ot/Psic">
    <rdf:type rdf:resource="http://www.w3.org/2002/07/owl#Class"/>
    <rdfs:label xml:lang="pt">Psicologia
Psicanálise
Psiquiatria</rdfs:label>
  </rdf:Description>
</rdf:RDF>
